

Implicit Differentiation :-

$$\left. \begin{aligned} y &= x^2 + 3 \checkmark \\ y &= \sin(x) \\ y &= \sqrt{1-x^2} \\ y &= \tan\left(\frac{1}{x^2+1}\right) \end{aligned} \right\}$$

Explicit form of a function.

$$\begin{aligned} \frac{dy}{dx} &= \frac{d}{dx}(x^2+3) \\ &= 2x+0=2x \end{aligned}$$

Implicit

$$xy=2 \rightarrow y = \frac{2}{x} \checkmark \quad \frac{dy}{dx} = \frac{d}{dx}\left(\frac{2}{x}\right) = -\frac{2}{x^2}$$

Explicit form.

$y(x)$ relation

$$x^2+y^2=2 \rightarrow y = \pm \sqrt{1-x^2}$$

$$x^2-2y^3+4y=2 \rightarrow y=?$$

$$y = \sin(x^2+y^2) \rightarrow y=?$$

$$\sqrt{x+1} = x-2y \rightarrow y=?$$

Implicit Differentiation:

$$\frac{x^2}{2} + \frac{y^2}{5} = 1$$

$$\frac{dy}{dx}=?$$

$$x^2+y^2=1$$

$$\frac{dy}{dx}$$



General Power Rule

$$\frac{d}{dx} \left((f(x))^n \right) = n (f(x))^{n-1} f'(x)$$

$y \rightarrow$ function of x

$$(x^n)' = n x^{n-1}$$

$$\frac{d}{dx} (y^n) = n y^{n-1} y'$$

$$\left\{ \begin{aligned} \frac{d}{dx} \left((f(y))^n \right) &= n (f(y))^{n-1} \frac{d}{dx} (f(y)) \\ &= n (f(y))^{n-1} f'(y) y' \end{aligned} \right\} \times$$

$$\frac{d}{dx} (\sin(y)) = \cos(y) \frac{dy}{dx}$$

$$\frac{d}{dx} (\cos(y)) = -\sin(y) y'$$

$$\frac{d}{dx} (\tan(y)) = \sec^2(y) y'$$

$$\frac{d}{dx} (f(y)) = f'(y) y'$$

$$\frac{d}{dx} (y^2 + 3y + \sin(y) - 3x)$$

$$= \frac{d}{dx} (y^2) + 3 \frac{d}{dx} (y) + \frac{d}{dx} (\sin y) - 3 \frac{d}{dx} (x)$$

$$= 2y \frac{dy}{dx} + 3 \frac{dy}{dx} + \cos(y) \frac{dy}{dx} - 3(1)$$

$$= 2y y' + 3 y' + (\cos y) y' - 3$$

E_{x2}

$$\frac{d}{dx} (xy^2)$$

$$= \frac{d}{dx}(x) y^2 + x \frac{d}{dx}(y^2)$$

$$= y^2 + x (2y y')$$

$$= y^2 + 2xyy'$$

$$y^3 + y^2 - 5y - x^2 = -4$$

$$\frac{d}{dx} (y^3 + y^2 - 5y - x^2) = \frac{d}{dx} (-4)$$

$$\frac{d}{dx}(y^3) + \frac{d}{dx}(y^2) - 5 \frac{dy}{dx} - \frac{d}{dx}(x^2) = 0$$

$$3y^2 y' + 2y y' - 5y' - 2x = 0$$

$$y' (3y^2 + 2y - 5) = 2x$$

$$y' = \frac{2x}{3y^2 + 2y - 5}$$

$$\frac{dy}{dx} = ?$$

$$2 \sin(x) \cos(y) = 1$$

$$\frac{dy}{dx} = ?$$

$$y = ?$$

$$\frac{d}{dx} (2 \sin(x) \cos(y)) = \frac{d}{dx} (1)$$

$$2 \frac{d}{dx} \left(\underbrace{\sin(x)}_f \underbrace{\cos(y)}_g \right) = 0$$

$$\cos(x) \cos(y) + \sin(x) \left(-\sin(y) \right) \frac{dy}{dx} = 0$$

$$\cos(x) \cos(y) - (\sin(x) \sin(y)) y' = 0$$

$$\cos x \cos y = \sin x \sin y y'$$

$$y' = \frac{\cos(x) \cos(y)}{\sin(x) \sin(y)} = \cot(x) \cot(y)$$

$$y' = \cot(x) \cot(y)$$

$$\frac{dy}{dx} = \cot(x) \cot(y)$$

$$\sqrt{xy} = x - 2y$$

$$\Rightarrow (xy)^{\frac{1}{2}} = x - 2y$$

$$\Rightarrow \frac{d}{dx} \left((xy)^{\frac{1}{2}} \right) = \frac{d}{dx} (x - 2y)$$

$$\Rightarrow \frac{1}{2} (xy)^{\frac{1}{2}-1} \frac{d}{dx} (xy) = 1 - 2y'$$

$$\Rightarrow \frac{1}{2 (xy)^{1/2}} \left[\frac{d}{dx} (xy) \right] = 1 - 2y'$$

$$\Rightarrow \frac{1}{2\sqrt{xy}} \left[(1)y + x y' \right] = 1 - 2y'$$

$$\Rightarrow \frac{y + x y'}{2\sqrt{xy}} = 1 - 2y'$$

$$\Rightarrow y + xy' = (1-2y')(2\sqrt{xy})$$

$$\Rightarrow \checkmark y + \checkmark xy' = \checkmark 2\sqrt{xy} - \checkmark 2y'\sqrt{xy}$$

$$\Rightarrow xy' + 2y'\sqrt{xy} = 2\sqrt{xy} - y$$

$$\Rightarrow y'(x + 2\sqrt{xy}) = 2\sqrt{xy} - y$$

$$\Rightarrow y' = \frac{2\sqrt{xy} - y}{x + 2\sqrt{xy}} \checkmark$$

$$3(x^2$$

$$\odot 3(x^2 + y^2)^2 = 100xy \checkmark$$

$$(3,1)$$

Equation of tangent
to - at (3,1)

$$\frac{d}{dx} [3(x^2 + y^2)^2] = \frac{d}{dx} (100xy)$$

$$\Rightarrow 3 \frac{d}{dx} ((x^2 + y^2)^2) = 100 \frac{d}{dx} (xy)$$

$$\odot$$

$$\Rightarrow 3 \left[2(x^2 + y^2) \frac{d}{dx} (x^2 + y^2) \right] = 100 \left[(1)y + x y' \right]$$

$$\Rightarrow 3 \left[2(x^2 + y^2)(2x + 2y y') \right] = 100(y + x y') \quad (3,1)$$

$$\Rightarrow 3 \left[2(9+1)(6+2y') \right] = 100(1+3y')$$

$$\Rightarrow 60(6+2y') = 100 + 300y'$$

$$\Rightarrow 360 + 120y' = 100 + 300y'$$

$$\Rightarrow 260 = 180y'$$

$$\Rightarrow y' = \frac{13}{9}$$

$$m = \frac{13}{9} \text{ at } (3,1) \text{ to } \underline{\quad}$$

$$(3, 1)$$

$$m = \frac{13}{9}$$

$$y - 1 = \frac{13}{9}(x - 3)$$

$$9y - 9 = 13x - 39$$

$$9y - 13x = -30$$

⑦

$$\frac{dy}{dx} = ?$$

$$y = \tan(x^2 + y^2)$$

$$\frac{dy}{dx} = ?$$

$$x = 0, y = 0$$

$$\frac{dy}{dx} = \frac{d}{dx}(\tan(x^2 + y^2))$$

$$y' = (\sec^2(x^2 + y^2)) \frac{d}{dx}(x^2 + y^2)$$

$$y' = (\sec^2(x^2 + y^2))(2x + 2yy')$$

$$y' = (\sec^2(0))(0 + 0)$$

$$y' = 0$$

$$m = 0$$

$$m = 0,$$

$$x = 0,$$

$$y = 0$$

$$(0, 0)$$

$$y - 0 = 0(x - 0)$$

$$y = 0$$

$$(x^2 + y^2)$$

$$\textcircled{c} \quad (x^2 + y^2 - 1)^3 = x^2 y^3 \quad \frac{dy}{dx} = \quad x=1, y=0$$

$$\Rightarrow \frac{d}{dx} \left((x^2 + y^2 - 1)^3 \right) = \frac{d}{dx} (x^2 y^3)$$

$$\Rightarrow 3(x^2 + y^2 - 1)^2 \frac{d}{dx} (x^2 + y^2 - 1) = (2x)y^3 + x^2(3y^2 y')$$

$$\Rightarrow 3(x^2 + y^2 - 1)^2 (2x + 2yy' - 0) = 2xy^3 + 3x^2 y^2 y'$$

$$\Rightarrow 3(1 + 0 - 1) (2(1) + 2(0)y') = 2(1)(0)^3$$

$$(x^2 + y^2 - 1)^3 = x^2 y^3$$

$$\Rightarrow \frac{d}{dx} \left((x^2 + y^2 - 1)^3 \right) = \frac{d}{dx} (x^2 y^3)$$

$$\Rightarrow 3(x^2 + y^2 - 1)^2 \frac{d}{dx} (x^2 + y^2 - 1) = (2x)y^3 + x^2(3y^2 y')$$

$$\Rightarrow \underline{3(x^2 + y^2 - 1)^2 (2x + 2yy')} = 2xy^3 + 3x^2 y^2 y'$$

$$\Rightarrow \underline{6x(x^2 + y^2 - 1)^2 + 6yy'(x^2 + y^2 - 1)^2} = 2xy^3 + \underline{3x^2 y^2 y'}$$

$$\Rightarrow 6yy'(x^2 + y^2 - 1)^2 - 3x^2 y^2 y' = 2xy^3 - 6x(x^2 + y^2 - 1)^2$$

$$\Rightarrow y^2 (6y(x^2 + y^2 - 1)^2 - 3x^2 y^2) = 2xy^3 - 6(x^2 + y^2 - 1)^2$$

$$\Rightarrow \frac{dy}{dx} = \frac{2xy^3 - 6(x^2 + y^2 - 1)^2}{6y(x^2 + y^2 - 1)^2 - 3x^2 y^2}$$

